fuse Write into Base

src/lowparse/pulse/LowParse.Pulse.Base.fst
@@ -6,6 +6,7 @@ open LowParse.Spec.Base
 
 module SZ = FStar.SizeT
 module Trade = Pulse.Lib.Trade.Util
+module S = Pulse.Lib.Slice
 
 let pts_to_serialized (#k: parser_kind) (#t: Type) (#p: parser k t) (s: serializer p) (input: slice byte) (#[exact (`1.0R)] pm: perm) (v: t) : slprop =
   pts_to input #pm (bare_serialize s v)
@@ -652,5 +653,220 @@ fn reader_of_leaf_reader
 {
   let x = r input #pm #v;
   f x
+}
+```
+
+inline_for_extraction
+let l2r_writer
+  (#t' #t: Type0)
+  (vmatch: t' -> t -> slprop)
+  (#k: parser_kind)
+  (#p: parser k t)
+  (s: serializer p)
+= (x': t') ->
+  (#x: Ghost.erased t) ->
+  (out: slice byte) ->
+  (offset: SZ.t) ->
+  (#v: Ghost.erased bytes) ->
+  stt SZ.t
+    (S.pts_to out v ** vmatch x' x ** pure (
+      SZ.v offset + Seq.length (bare_serialize s x) <= Seq.length v
+    ))
+    (fun res -> exists* v' .
+      S.pts_to out v' ** vmatch x' x ** pure (
+      let bs = bare_serialize s x in
+      SZ.v offset + Seq.length bs <= Seq.length v /\
+      Seq.length v' == Seq.length v /\
+      Seq.slice v' 0 (SZ.v offset) == Seq.slice v 0 (SZ.v offset) /\
+      Seq.slice v' (SZ.v offset) (SZ.v offset + Seq.length bs) == bs
+    ))
+
+```pulse
+fn l2r_writer_ext
+  (#t' #t: Type0)
+  (#vmatch: t' -> t -> slprop)
+  (#k1: Ghost.erased parser_kind)
+  (#p1: parser k1 t)
+  (#s1: serializer p1)
+  (w: l2r_writer vmatch s1)
+  (#k2: Ghost.erased parser_kind)
+  (#p2: parser k2 t)
+  (s2: serializer p2 { forall b . parse p1 b == parse p2 b })
+: l2r_writer #t' #t vmatch #k2 #p2 s2
+= (x': t')
+  (#x: Ghost.erased t)
+  (out: slice byte)
+  (offset: SZ.t)
+  (#v: Ghost.erased bytes)
+{
+  serializer_unique_strong s1 s2 x;
+  w x' out offset
+}
+```
+
+inline_for_extraction
+```pulse
+fn l2r_writer_lens
+  (#t1' #t2' #t: Type0)
+  (vmatch1: t1' -> t -> slprop)
+  (vmatch2: t2' -> t -> slprop)
+  (lens: (x2': t2') -> (x: Ghost.erased t) -> stt t1'
+    (vmatch2 x2' x)
+    (fun x1' -> vmatch1 x1' x ** trade (vmatch1 x1' x) (vmatch2 x2' x))
+  )
+  (#k: parser_kind)
+  (#p: parser k t)
+  (#s: serializer p)
+  (w: l2r_writer vmatch1 s)
+: l2r_writer #t2' #t vmatch2 #k #p s
+= (x2': t2')
+  (#x: Ghost.erased t)
+  (out: slice byte)
+  (offset: SZ.t)
+  (#v: Ghost.erased bytes)
+{
+  let x1' = lens x2' _;
+  let res = w x1' out offset;
+  elim_trade _ _;
+  res
+}
+```
+
+inline_for_extraction
+let compute_remaining_size
+  (#t' #t: Type0)
+  (vmatch: t' -> t -> slprop)
+  (#k: parser_kind)
+  (#p: parser k t)
+  (s: serializer p)
+= (x': t') ->
+  (#x: Ghost.erased t) ->
+  (out: R.ref SZ.t) ->
+  (#v: Ghost.erased SZ.t) ->
+  stt bool
+    (R.pts_to out v ** vmatch x' x)
+    (fun res -> exists* v' .
+      R.pts_to out v' ** vmatch x' x ** pure (
+      let bs = Seq.length (bare_serialize s x) in
+      (res == true <==> bs <= SZ.v v) /\
+      (res == true ==> bs + SZ.v v' == SZ.v v)
+    ))
+
+inline_for_extraction
+```pulse
+fn compute_size
+  (#t' #t: Type0)
+  (#vmatch: t' -> t -> slprop)
+  (#k: Ghost.erased parser_kind)
+  (#p: parser k t)
+  (#s: serializer p)
+  (cr: compute_remaining_size vmatch s)
+  (x': t')
+  (#x: Ghost.erased t)
+  (out: R.ref SZ.t)
+  (#v: Ghost.erased SZ.t)
+  requires
+    (R.pts_to out v ** vmatch x' x)
+  returns res: bool
+  ensures exists* v' .
+      R.pts_to out v' ** vmatch x' x ** pure (
+      let bs = Seq.length (bare_serialize s x) in
+      (res == true <==> bs <= SZ.v v) /\
+      (res == true ==> bs == SZ.v v')
+    )
+{
+  let capacity = !out;
+  let res = cr x' out;
+  if res {
+    let remaining = !out;
+    out := SZ.sub capacity remaining;
+    true
+  } else {
+    false
+  }
+}
+```
+
+inline_for_extraction
+```pulse
+fn compute_remaining_size_ext
+  (#t' #t: Type0)
+  (#vmatch: t' -> t -> slprop)
+  (#k1: Ghost.erased parser_kind)
+  (#p1: parser k1 t)
+  (#s1: serializer p1)
+  (cr1: compute_remaining_size vmatch s1)
+  (#k2: Ghost.erased parser_kind)
+  (#p2: parser k2 t)
+  (s2: serializer p2 {
+    forall b . parse p1 b == parse p2 b
+  })
+: compute_remaining_size #t' #t vmatch #k2 #p2 s2
+=
+  (x': t')
+  (#x: Ghost.erased t)
+  (out: R.ref SZ.t)
+  (#v: Ghost.erased SZ.t)
+{
+  serializer_unique_strong s1 s2 x;
+  cr1 x' out
+}
+```
+
+inline_for_extraction
+```pulse
+fn compute_remaining_size_lens
+  (#t1' #t2' #t: Type0)
+  (vmatch1: t1' -> t -> slprop)
+  (vmatch2: t2' -> t -> slprop)
+  (lens: (x2': t2') -> (x: Ghost.erased t) -> stt t1'
+    (vmatch2 x2' x)
+    (fun x1' -> vmatch1 x1' x ** trade (vmatch1 x1' x) (vmatch2 x2' x))
+  )
+  (#k: parser_kind)
+  (#p: parser k t)
+  (#s: serializer p)
+  (w: compute_remaining_size vmatch1 s)
+: compute_remaining_size #t2' #t vmatch2 #k #p s
+=
+  (x2': t2')
+  (#x: Ghost.erased t)
+  (out: R.ref SZ.t)
+  (#v: Ghost.erased SZ.t)
+{
+  let x1' = lens x2' _;
+  let res = w x1' out;
+  elim_trade _ _;
+  res
+}
+```
+
+inline_for_extraction
+```pulse
+fn compute_remaining_size_constant_size
+  (#t' #t: Type0)
+  (#vmatch: t' -> t -> slprop)
+  (#k: Ghost.erased parser_kind)
+  (#p: parser k t)
+  (s: serializer p)
+  (sz: SZ.t {
+    k.parser_kind_high == Some k.parser_kind_low /\
+    k.parser_kind_low == SZ.v sz
+  })
+: compute_remaining_size #t' #t vmatch #k #p s
+=
+  (x': t')
+  (#x: Ghost.erased t)
+  (out: R.ref SZ.t)
+  (#v: Ghost.erased SZ.t)
+{
+  serialize_length s x;
+  let capacity = !out;
+  if (SZ.lt capacity sz) {
+    false
+  } else {
+    out := SZ.sub capacity sz;
+    true
+  }
 }
 ```
